Heap/test.v
@@ -1,8 +1,0 @@
-Require Import PL.Monad.
-Require Import PL.Monad.
-Import SetsNotation
-       KleeneFix Sets_CPO
-       Monad
-       MonadNotation.
-
-Check bind.
